src/Values.v
@@ -1,5 +1,6 @@
 Require Import AST.
 Require Import String.
+Require Import Coqlib.
 
 Inductive val :=
 | bit (b : bool) (* Can we ever get this now? *)
@@ -12,14 +13,16 @@ Inductive val :=
 | vcons (v : val) (e : Expr) (E : ident -> option val) (* lazy list: first val computed, rest is thunked *)
 | vnil (* empty list *)
 | vcomp (e : Expr) (E : ident -> option val) (l : list (list Match)) (* lazy list comprehension *)
-| vapp (t1 t2 t3 : Typ) (l1 l2 : Expr) (E : ident -> option val) (* list append *)
-| vsplit (t1 t2 t3 : Typ) (l : Expr) (E : ident -> option val)
-| vsplitAt (t1 t2 t3 : Typ) (l : Expr) (E : ident -> option val)
-
+| vapp (l1 l2 : Expr) (E : ident -> option val)
+| vsplit (n m : Z) (l : Expr) (E : ident -> option val)
+(*| vsplitAt (t1 t2 t3 : Typ) (l : Expr) (E : ident -> option val)*)
 (* a slice of an underlying list *)
 (* NOTE: indexing into slices can be a bit wonky *)
 (* you can slice l from 3 to 6 *)
 (* then, access 1 would actually go to element 4 of l *)
 (* only then would you do any computation on the lazy list *)
-| vslice (l h : nat) (e : Expr) (E : ident -> option val) 
+| vslice (l h : nat) (e : Expr) (E : ident -> option val)
 .
+
+Definition env := ident -> option val.
+Definition empty : env := fun _ => None.
