verif/SplitTestA.v
@@ -1,0 +1,50 @@
+Require Import List.
+Import ListNotations.
+Require Import String.
+
+(* Borrow from CompCert *)
+Require Import Coqlib.
+Require Import Bitvectors.
+
+Require Import AST.
+Require Import Semantics.
+Require Import Utils.
+Require Import Builtins.
+Require Import BuiltinSem.
+Require Import Values.        
+
+Require Import EvalTac.
+Require Import SplitTest.
+
+Lemma eval_a :
+  eval_expr ge empty a (bits (v 1)).
+Proof.
+  g.
+  e. e. e. e. e. g.
+  e. e. e. e. e. e. e. e. e. g.
+  e. e. e. e. g.
+  e. e. e. e. g.
+  e. e. e. e. g.
+  e. e. e. repeat e. e.
+  repeat e.
+  e. e. e. e. g.
+  e. e. e. repeat e. e.
+  repeat e. 
+  e. e. e. e.
+  e. e. e. e. e. e.
+  e. e. e. e. g.
+  e. e. e. e. e. e. e. e.
+  e. e. repeat e. e.
+  eapply select_split. e. reflexivity.
+  simpl. reflexivity.
+  e. e. e. g.
+  e. e. e. e. e. e. e. e.
+  e.
+  e. repeat e.
+  e. eapply select_slice.
+  repeat e. reflexivity.
+  simpl. repeat e.
+  Unshelve.
+  all: exact nz.
+Qed.  
+  
